theories/ftlr/Store.v
@@ -28,185 +28,33 @@ Section fundamental.
   Implicit Types w : (leibnizO Word).
   Implicit Types interp : (D).
 
-  (* The necessary resources to close the region again,
-      except for the points to predicate, which we will store separately *)
-  (* Definition region_open_resources W l ls p φ (v : Word): iProp Σ := *)
-  (*   (∃ ρ, *)
-  (*       sts_state_std l ρ *)
-  (*       ∗ ⌜std W !! l = Some ρ⌝ *)
-  (*       ∗ ⌜ρ ≠ Revoked⌝ *)
-  (*       ∗ ⌜(∀ g, ρ ≠ Frozen g)⌝ *)
-  (*       ∗ open_region_many (l :: ls) W *)
-  (*       ∗ rel l p φ)%I. *)
+  Definition wcond' (P : D) p g b e a r : iProp Σ
+    := (if decide (writeAllowed_in_r_a (<[PC:= WCap p g b e a]> r) a)
+        then □ (∀ W0 (w : Word), interp W0 w -∗ P W0 w)
+        else emp)%I.
+  Instance wcond'_pers P p g b e a r: Persistent (wcond' P p g b e a r).
+  Proof. intros. rewrite /wcond'. case_decide;apply _. Qed.
 
-
-  Definition later_zcond (P : D) (has_later : bool) :=
-    if has_later
-    then (▷ □ ∀ W1 W2 (z : Z), P W1 (WInt z) -∗ P W2 (WInt z))%I
-    else (□ ∀ W1 W2 (z : Z), P W1 (WInt z) -∗ P W2 (WInt z))%I.
-
-  Definition later_wcond (P : D) (has_later : bool) :=
-    if has_later
-    then ( ▷ □ ∀ W (w : Word), interp W w -∗ P W w)%I
-    else ( □ ∀ W (w : Word), interp W w -∗ P W w)%I.
-
-  Definition later_rcond (P : D) (has_later : bool):=
-    if has_later
-    then ( ▷ □ ∀ W (w : Word), P W w -∗ interp W w)%I
-    else ( □ ∀ W (w : Word), P W w -∗ interp W w)%I.
-
-  Lemma P_zcond_monotone_generalZ
-    (W : WORLD) (ρ : region_type) (p : Perm) (a : Addr) (z : Z) (P : D) :
-    std W !! a = Some ρ →
-    later_zcond P false -∗
-    monotonicity_guarantees_region ρ (WInt z) p (λ Wv : WORLD * (leibnizO Word), (P Wv.1) Wv.2).
+  Lemma storev_interp_mono W (r : Reg) (r1 : RegName) (r2 : Z + RegName) p g b e a p' ρ storev:
+     PermFlows p p'
+    -> word_of_argument r r2 = Some storev
+    → reg_allows_store r r1 p g b e a storev
+    → std W !! a = Some ρ
+    → interp W (WCap p g b e a)
+    -∗ monotonicity_guarantees_region ρ storev p'
+         (λ Wv : WORLD * (leibnizO Word), (interp Wv.1) Wv.2).
   Proof.
-    unfold monotonicity_guarantees_region.
-    iIntros (Hstd) "#Hzcond".
-    destruct ρ;auto.
-    - destruct (pwl p) eqn: HpwlP1 ; iModIntro; simpl; iIntros (W0 W1) "% HIW0".
-      all: by iApply "Hzcond".
-    - iModIntro; simpl; iIntros (W0 W1) "% HIW0".
-      by iApply "Hzcond".
+    iIntros (Hflp Hwoa Hras Hststd) "HInt".
+    destruct Hras as (Hrir & Hwa & Hwb & Hloc).
+    destruct storev as [z | sb | ot sb ].
+    - iApply (interp_monotone_generalZ with "[HInt]" ); eauto.
+    - destruct sb ;
+        [ iApply (interp_monotone_generalW with "[HInt]" )
+        | iApply (interp_monotone_generalSr with "[HInt]" )]
+      ; eauto.
+    - iApply (interp_monotone_generalSd with "[HInt]" ); eauto.
   Qed.
 
-Lemma P_monotone_generalSd (W : WORLD) (ρ : region_type)
-  (p p' : Perm) (g : Locality) (b e a : Addr)
-  (ot : OType) (sb : Sealable) (P : D) :
-  std W !! a = Some ρ →
-  withinBounds b e a = true →
-  PermFlows p p' →
-  ((fixpoint interp1) W) (WCap p g b e a)
-  -∗ ((fixpoint interp1) W) (WSealed ot sb)
-  -∗ later_wcond P false
-  -∗ monotonicity_guarantees_region ρ (WSealed ot sb) p' (λ Wv : WORLD * (leibnizO Word), (P Wv.1) Wv.2).
-Proof.
-  unfold monotonicity_guarantees_region.
-  iIntros (Hstd Hwb Hfl') "#Hvdst #Hvsrc #Hwcond".
-  destruct ρ;auto.
-  - destruct (pwl p') eqn: Hpwlp' ; iModIntro; simpl; iIntros (W0 W1) "% HIW0".
-    + iApply "Hwcond"; rewrite !fixpoint_interp1_eq; iEval (cbn) in "Hvsrc"; iEval (cbn); done.
-    + iApply "Hwcond"; rewrite !fixpoint_interp1_eq; iEval (cbn) in "Hvsrc"; iEval (cbn); done.
-  - iModIntro; simpl; iIntros (W0 W1) "% HIW0".
-    iApply "Hwcond"; rewrite !fixpoint_interp1_eq; iEval (cbn) in "Hvsrc"; iEval (cbn); done.
-Qed.
-
-Lemma P_monotone_generalSr (W : WORLD) (ρ : region_type)
-  (p p' : Perm) (g : Locality) (b e a : Addr)
-  (sp : SealPerms) (sg : Locality) (sb se sa : OType) (P:D) :
-  std W !! a = Some ρ →
-  withinBounds b e a = true →
-  PermFlows p p' →
-  ((fixpoint interp1) W) (WCap p g b e a)
-  -∗ ((fixpoint interp1) W) (WSealRange sp sg sb se sa)
-  -∗ later_wcond P false
-  -∗ monotonicity_guarantees_region ρ (WSealRange sp sg sb se sa) p' (λ Wv : WORLD * (leibnizO Word), (P Wv.1) Wv.2).
-Proof.
-  unfold monotonicity_guarantees_region.
-  iIntros (Hstd Hwb Hfl') "#Hvdst #Hvsrc #Hwcond".
-  destruct ρ;auto.
-  - destruct (pwl p') eqn: Hpwlp' ; iModIntro; simpl; iIntros (W0 W1) "% HIW0".
-    + iApply "Hwcond"; rewrite !fixpoint_interp1_eq; iEval (cbn) in "Hvsrc"; iEval (cbn); done.
-    + iApply "Hwcond"; rewrite !fixpoint_interp1_eq; iEval (cbn) in "Hvsrc"; iEval (cbn); done.
-  - iModIntro; simpl; iIntros (W0 W1) "% HIW0".
-    iApply "Hwcond"; rewrite !fixpoint_interp1_eq; iEval (cbn) in "Hvsrc"; iEval (cbn); done.
-Qed.
-
-Lemma P_monotone_generalW (W : WORLD)  (ρ : region_type)
-  (p p' p'' : Perm) (g g' : Locality) (b e a b' e' a' : Addr) (P:D) :
-  std W !! a' = Some ρ →
-  withinBounds b' e' a' = true →
-  PermFlows p' p'' →
-  canStore p' (WCap p g b e a) = true →
-  ((fixpoint interp1) W) (WCap p' g' b' e' a')
-  -∗ ((fixpoint interp1) W) (WCap p g b e a)
-  -∗ later_wcond P false
-  -∗ monotonicity_guarantees_region ρ (WCap p g b e a) p''
-    (λ Wv : WORLD * (leibnizO Word), (P Wv.1) Wv.2).
-Proof.
-  unfold monotonicity_guarantees_region.
-  iIntros (Hstd Hwb Hfl' Hconds) "#Hvdst #Hvsrc #Hwcond".
-  destruct ρ;simpl;auto.
-  - destruct (pwl p'') eqn: HpwlP'' ; iModIntro; simpl;auto; iIntros (W0 W1) "% HIW0".
-    * iApply "Hwcond".
-      iApply interp_monotone; eauto.
-    * destruct g; first by iApply interp_monotone_nl.
-    (* The below case is a contradiction, since if g is local,
-      p' must be WL and p' flows into the non-WL p''*)
-      destruct p' ; try (simpl in Hconds; by exfalso).
-      all:destruct p'' eqn:Hp''v ; (by exfalso).
-  - iModIntro; iIntros (W0 W1) "% HIW0".
-    destruct g.
-    + by iApply interp_monotone_nl.
-    + (*Trick here: value relation leads to a contradiction if p' is WL,
-        since then its region cannot be permanent *)
-      iDestruct ( writeLocalAllowed_valid_cap_implies with "Hvdst" ) as %Ha; eauto.
-      by rewrite Hstd in Ha.
-Qed.
-
-  Lemma monotonicity_guarantees_wf (P : D) ρ w p :
-    later_rcond P false
-    -∗ later_wcond P false
-       -∗ monotonicity_guarantees_region
-            ρ w p (λ Wv : WORLD * (leibnizO Word), (interp Wv.1) Wv.2)
-          -∗ monotonicity_guarantees_region
-               ρ w p (λ Wv : WORLD * (leibnizO Word), (P Wv.1) Wv.2).
-  Proof.
-    iIntros "#Hrcond #Hwcond HmonoV"; cbn.
-    rewrite /monotonicity_guarantees_region.
-    destruct ρ; auto.
-    destruct (pwl p); auto; iDestruct "HmonoV" as "#HmonoV".
-    - iModIntro. iIntros (W0 W1 Hrelated) "HP".
-      iApply "Hwcond".
-      iApply "HmonoV"; auto.
-      iApply "Hrcond".
-      done.
-    - iModIntro. iIntros (W0 W1 Hrelated) "HP".
-      iApply "Hwcond".
-      iApply "HmonoV"; auto.
-      iApply "Hrcond".
-      done.
-    - iDestruct "HmonoV" as "#HmonoV".
-      iModIntro. iIntros (W0 W1 Hrelated) "HP".
-      iApply "Hwcond".
-      iApply "HmonoV"; auto.
-      iApply "Hrcond".
-      done.
-    Qed.
-
-
-  (* Lemma storev_P_mono W (r : Reg) (r1 : RegName) (r2 : Z + RegName) p g b e a p' ρ storev: *)
-  (*    PermFlows p p' *)
-  (*   -> word_of_argument r r2 = Some storev *)
-  (*   → reg_allows_store r r1 p g b e a storev *)
-  (*   → std W !! a = Some ρ *)
-  (*   → (fixpoint interp1) W (WCap p g b e a) *)
-  (*   (* -∗ (fixpoint interp1) W storev *) *)
-  (*   (* -∗ later_zcond P false *) *)
-  (*   (* -∗ (if writeAllowed p' then later_wcond P false else True) *) *)
-  (*   (* -∗ (if readAllowed p' then later_rcond P false else True) *) *)
-  (*   -∗ ∃ (P:D), *)
-  (*       ⌜persistent_cond P⌝ *)
-  (*       ∗ zcond P *)
-  (*       ∗ rcond P interp *)
-  (*       ∗ wcond P interp *)
-  (*       ∗ monotonicity_guarantees_region ρ storev p' *)
-  (*        (λ Wv : WORLD * (leibnizO Word), (P Wv.1) Wv.2). *)
-  (* Proof. *)
-  (*   iIntros (Hflp Hwoa Hras Hststd) "HInt". *)
-  (*   destruct Hras as (Hrir & Hwa & Hwb & Hloc). *)
-  (*   rewrite /monotonicity_guarantees_region. *)
-  (*   destruct storev as [z | sb | ot sb ]. *)
-  (*   (* - iApply (P_zcond_monotone_generalZ with "[HInt]" ); eauto. *) *)
-  (*   (* - admit. *) *)
-  (*   (* - rewrite /monotonicity_guarantees_region. *) *)
-  (*   (*   destruct ρ;auto. *) *)
-  (*   (*   2: { iModIntro; simpl; iIntros (W0 W1) "% HIW0". *) *)
-  (*   (*        replace (writeAllowed p') with true; last admit. *) *)
-  (*   (*        iApply "Hwcond". *) *)
-  (*   (*        admit. *) *)
-  (*   (*   } *) *)
-  (* Abort. *)
 
   Lemma interp_hpf_eq (W : WORLD) P (regs : leibnizO Reg) (r1 : RegName)
     p g b e a pc_p pc_g pc_b pc_e pc_p' w storev:
@@ -231,53 +79,21 @@ Qed.
       done.
   Qed.
 
-  Lemma storev_interp_mono W (r : Reg) (r1 : RegName) (r2 : Z + RegName) p g b e a p' ρ storev:
-     PermFlows p p'
-    -> word_of_argument r r2 = Some storev
-    → reg_allows_store r r1 p g b e a storev
-    → std W !! a = Some ρ
-    → ((fixpoint interp1) W) (WCap p g b e a)
-    -∗ monotonicity_guarantees_region ρ storev p'
-         (λ Wv : WORLD * (leibnizO Word), (interp Wv.1) Wv.2).
-  Proof.
-    iIntros (Hflp Hwoa Hras Hststd) "HInt".
-    destruct Hras as (Hrir & Hwa & Hwb & Hloc).
-    destruct storev as [z | sb | ot sb ].
-    - iApply (interp_monotone_generalZ with "[HInt]" ); eauto.
-    - destruct sb ;
-        [ iApply (interp_monotone_generalW with "[HInt]" )
-        | iApply (interp_monotone_generalSr with "[HInt]" )]
-      ; eauto.
-    - iApply (interp_monotone_generalSd with "[HInt]" ); eauto.
-  Qed.
-
-  Lemma storev_P_mono W P (r : Reg) (r1 : RegName) (r2 : Z + RegName) p g b e a p' ρ storev:
-     PermFlows p p'
-    -> word_of_argument r r2 = Some storev
-    → reg_allows_store r r1 p g b e a storev
-    → std W !! a = Some ρ
-    → ((fixpoint interp1) W) (WCap p g b e a)
-    -∗ later_rcond P false
-    -∗ later_wcond P false
-    -∗ monotonicity_guarantees_region ρ storev p'
-         (λ Wv : WORLD * (leibnizO Word), (P Wv.1) Wv.2).
-  Proof.
-    iIntros (Hflp Hwoa Hras Hststd) "#HInt #Hrcond #Hwcond".
-    iAssert
-     (monotonicity_guarantees_region ρ storev p'
-         (λ Wv : WORLD * (leibnizO Word), (interp Wv.1) Wv.2)) as "HmonoV".
-    { iApply storev_interp_mono ; eauto. }
-    iApply monotonicity_guarantees_wf; eauto.
-  Qed.
+(* Definition if_later_P' (b: bool) (P :  iProp Σ) := *)
+(*   (if b then ▷ P else P)%I. *)
 
 
-  Definition region_open_resources W l ls p φ (v : Word): iProp Σ :=
+  Definition region_open_resources W l ls p φ (v : Word) (P : D) (has_later : bool): iProp Σ :=
     (∃ ρ,
         sts_state_std l ρ
         ∗ ⌜std W !! l = Some ρ⌝
         ∗ ⌜ρ ≠ Revoked⌝
         ∗ ⌜(∀ g, ρ ≠ Frozen g)⌝
         ∗ open_region_many (l :: ls) W
+        ∗ if_later_P
+            has_later
+            (monotonicity_guarantees_region ρ v p (safeC P)
+             ∗ monotonicity_guarantees_regionFull ρ p (safeC P))
         ∗ rel l p φ)%I.
 
   Lemma store_inr_eq {regs r p0 g0 b0 e0 a0 p1 g1 b1 e1 a1 storev}:
@@ -290,12 +106,6 @@ Qed.
     destruct Hrar' as (Hinr0 & _). rewrite /read_reg_inr Hinr0 in H3.
     by inversion H3.
   Qed.
-
-  (* Lemma later_wcond_later_is_wcond (P:D) : *)
-  (*   later_wcond true P ∗-∗ wcond P interp. *)
-  (* Proof. *)
-  (*   iSplit; iIntros ; cbn ; done. *)
-  (* Qed. *)
 
   (* Description of what the resources are supposed to look like
      after opening the region if we need to,
@@ -310,31 +120,38 @@ Qed.
                     ⌜PermFlows p p'⌝
                     ∗ ⌜ persistent_cond P' ⌝
                     ∗ a ↦ₐ w
-                    ∗ later_zcond P' has_later
-                    ∗ (if writeAllowed p' then later_wcond P' has_later else True)
-                    ∗ (if readAllowed p' then later_rcond P' has_later else True)
-                    ∗ (region_open_resources W a [pc_a] p'
-                         (λ Wv : WORLD * (leibnizO Word), (P' Wv.1) Wv.2) w)
+                    ∗ if_later_P has_later (zcond P')
+                    ∗ (if writeAllowed p'
+                       then if_later_P has_later (wcond P' interp)
+                       else True)
+                    ∗ (if readAllowed p'
+                       then if_later_P has_later (rcond P' interp)
+                       else True)
+                    ∗ (region_open_resources W a [pc_a] p' (safeC P') w P' has_later)
                 else open_region pc_a W ∗ ⌜PermFlows p pc_p⌝  )
           else open_region pc_a W)%I.
 
   Definition allow_store_mem W r1 r2 (regs : Reg) pc_a (pc_p : Perm) pc_w (mem : Mem)
     (has_later : bool) :=
-    (∃ p g b e a storev, ⌜read_reg_inr regs r1 p g b e a⌝
-                         ∗ ⌜word_of_argument regs r2 = Some storev⌝
-                         ∗ if decide (reg_allows_store regs r1 p g b e a storev)
-                           then (if decide (a ≠ pc_a)
-                                 then ∃ p' (P':D) w,
-                                     ⌜PermFlows p p'⌝
-                                     ∗ ⌜ persistent_cond P' ⌝
-                                     ∗ later_zcond P' has_later
-                                     ∗ (if writeAllowed p' then later_wcond P' has_later else True)
-                                     ∗ (if readAllowed p' then later_rcond P' has_later else True)
-                                     ∗ ⌜mem = <[a:=w]> (<[pc_a:=pc_w]> ∅)⌝
-                                     ∗ (region_open_resources W a [pc_a] p'
-                                          (λ Wv : WORLD * (leibnizO Word), (P' Wv.1) Wv.2) w )
-                                 else  ⌜mem = <[pc_a:=pc_w]> ∅⌝ ∗ open_region pc_a W  ∗ ⌜PermFlows p pc_p⌝)
-                           else  ⌜mem = <[pc_a:=pc_w]> ∅⌝ ∗ open_region pc_a W)%I.
+    (∃ p g b e a storev,
+        ⌜read_reg_inr regs r1 p g b e a⌝
+        ∗ ⌜word_of_argument regs r2 = Some storev⌝
+        ∗ if decide (reg_allows_store regs r1 p g b e a storev)
+          then (if decide (a ≠ pc_a)
+                then ∃ p' (P':D) w,
+                    ⌜PermFlows p p'⌝
+                    ∗ ⌜ persistent_cond P' ⌝
+                    ∗ if_later_P has_later (zcond P')
+                    ∗ (if writeAllowed p'
+                       then if_later_P  has_later (wcond P' interp)
+                       else True)
+                    ∗ (if readAllowed p'
+                       then if_later_P  has_later (rcond P' interp)
+                       else True)
+                    ∗ ⌜mem = <[a:=w]> (<[pc_a:=pc_w]> ∅)⌝
+                    ∗ (region_open_resources W a [pc_a] p' (safeC P') w P' has_later)
+                else  ⌜mem = <[pc_a:=pc_w]> ∅⌝ ∗ open_region pc_a W  ∗ ⌜PermFlows p pc_p⌝)
+          else  ⌜mem = <[pc_a:=pc_w]> ∅⌝ ∗ open_region pc_a W)%I.
 
   Lemma create_store_res:
     ∀ (W : WORLD) (regs : leibnizO Reg)
@@ -379,13 +196,13 @@ Qed.
       destruct HH as [ρ' [Hstd' [Hnotrevoked' Hnotfrozen'] ] ].
       (* We can finally frame off Hsts here, since it is no longer needed after opening the region*)
       iDestruct (region_open_next _ _ _ a0 p'' ρ' with "[$Hrel'' $Hr $Hsts]")
-        as (w0) "($ & Hstate' & Hr & Ha0 & Hfuture & Hval)"; eauto.
+        as (w0) "($ & Hstate' & Hr & Ha0 & Hfuture & HfutureFull & Hval)"; eauto.
       { intros [g1 Hcontr];specialize (Hnotfrozen' g1); contradiction. }
       { apply not_elem_of_cons. split; auto. apply not_elem_of_nil. }
       iExists p'',P''.
-      iAssert ((if writeAllowed p'' then later_wcond P'' true else True)%I) as "Hwcond'".
+      iAssert ((if writeAllowed p'' then ▷ wcond P'' interp else True)%I) as "Hwcond'".
       { destruct (writeAllowed p''); done. }
-      iAssert ((if readAllowed p'' then later_rcond P'' true else True)%I) as "Hrcond'".
+      iAssert ((if readAllowed p'' then  ▷ rcond P'' interp else True)%I) as "Hrcond'".
       { destruct (readAllowed p''); done. }
 
       iFrame "∗#".
@@ -410,8 +227,9 @@ Qed.
     case_decide as Hallows.
     - case_decide as Haeq.
       + pose(Hallows' := Hallows). destruct Hallows as (Hrinr & Hra & Hwb & HLoc).
-        iDestruct "HStoreRes" as (p0' P0' w0 Hflp' HpersP0')
-                                   "(HStoreCh & #Hzcond & #Hwcond & #Hrcond & HStoreRest)".
+        iDestruct "HStoreRes"
+          as (p0' P0' w0 Hflp' HpersP0')
+               "(HStoreCh & #Hzcond & #Hwcond & #Hrcond & HStoreRest)".
         iExists _.
         iSplitL "HStoreRest".
         ++ iExists p1,g1,b1,e1,a1,storev. iFrame "%".
@@ -462,13 +280,6 @@ Qed.
   Qed.
 
 
-  Definition wcond' (P : D) p g b e a r : iProp Σ
-    := (if decide (writeAllowed_in_r_a (<[PC:= WCap p g b e a]> r) a)
-        then □ (∀ W0 (w : Word), interp W0 w -∗ P W0 w)
-        else emp)%I.
-  Instance wcond'_pers P p g b e a r: Persistent (wcond' P p g b e a r).
-  Proof. intros. rewrite /wcond'. case_decide;apply _. Qed.
-
   (* Note that we turn in all information that we might have on the monotonicity of the current PC value, so that in the proof of the ftlr case itself, we do not have to worry about whether the PC was written to or not when we close the last location pc_a in the region *)
    Lemma mem_map_recover_res:
     ∀ (W : WORLD) (regs : Reg)
@@ -483,14 +294,20 @@ Qed.
     -∗ (∀ (r1 : RegName) v, ⌜r1 ≠ PC⌝ → ⌜regs !! r1 = Some v⌝ → ((fixpoint interp1) W) v)
     -∗ ((fixpoint interp1) W) (WCap pc_p pc_g pc_b pc_e pc_a)
     -∗ P W pc_w
-    -∗ later_rcond P false
+    -∗ if_later_P false (rcond P interp)
     -∗ wcond' P pc_p pc_g pc_b pc_e pc_a regs
-    -∗ monotonicity_guarantees_region ρ pc_w pc_p' (λ Wv : WORLD * Word, P Wv.1 Wv.2)
+    -∗ monotonicity_guarantees_region ρ pc_w pc_p' (safeC P)
+    -∗ monotonicity_guarantees_regionFull ρ pc_p' (safeC P)
     -∗ ([∗ map] a0↦w0 ∈ <[a0 := storev]> mem0, a0 ↦ₐ w0)
-    -∗ ∃ v, open_region pc_a W ∗ pc_a ↦ₐ v ∗ P W v ∗ monotonicity_guarantees_region ρ v pc_p' (λ Wv : WORLD * Word, P Wv.1 Wv.2).
+    -∗ ∃ v,
+        open_region pc_a W
+        ∗ pc_a ↦ₐ v
+        ∗ P W v
+        ∗ monotonicity_guarantees_region ρ v pc_p' (safeC P)
+        ∗ monotonicity_guarantees_regionFull ρ pc_p' (safeC P).
    Proof.
     intros W regs pc_w r1 r2 p0 pc_p pc_p' g0 pc_g b0 e0 a0 pc_b pc_e pc_a mem0 oldv storev ρ P Hwoa Hras Hstdst Ha0.
-    iIntros "HStoreMem #Hreg #HVPCr Hpc_w #Hrcond #Hwcond Hpcmono Hmem".
+    iIntros "HStoreMem #Hreg #HVPCr Hpc_w #Hrcond #Hwcond Hpcmono HpcmonoFull Hmem".
     iDestruct "HStoreMem" as (p1 g1 b1 e1 a1 storev1) "[% [% HStoreRes] ]".
     destruct (store_inr_eq Hras H) as (<- & <- &<- &<- &<-).
     inversion H0; simplify_eq.
@@ -522,33 +339,27 @@ Qed.
     case_decide as Haeq.
     + iExists pc_w.
       destruct Hallows as [Hrinr [Hwa [Hwb Hloc] ] ].
-      iDestruct "HStoreRes" as (p' P' w' Hflp' HpersP') "(#Hzcond' & #Hwcond' & #Hrcond' & -> & HLoadRes)".
+      iDestruct "HStoreRes"
+        as (p' P' w' Hflp' HpersP') "(#Hzcond' & #Hwcond' & #Hrcond' & -> & HStoreRes)".
       rewrite lookup_insert in Ha0; inversion Ha0; clear Ha0; subst.
-      iDestruct "HLoadRes" as (ρ1) "(Hstate' & % & % & % & Hr & #Hrel')".
-
+      iDestruct "HStoreRes" as (ρ1) "(Hstate' & % & % & % & Hr & [#HmonoV #Hmono] & Hrel')".
       rewrite insert_insert memMap_resource_2ne; last auto.
       iDestruct "Hmem" as  "[Ha1 Hpc_a]".
       iFrame.
-      
-      (* iDestruct (storev_interp_mono with "HVr1") as "Hr1Mono"; eauto. *)
-      iDestruct ((storev_P_mono _ P') with "[HVr1] [Hwcond'] [Hrcond']")
-        as "HmonoP'"; eauto.
-      eauto.
-      eauto.
-      eauto.
-      eauto.
-      eauto.
-    iDestruct (region_close_next with "[$Hr $Ha1 $Hrel' $Hstate' HmonoP']") as "Hr"; eauto.
-    { intros [g Hcontr]. specialize (H2 g). done. }
-    { apply not_elem_of_cons; split; [auto|apply not_elem_of_nil]. }
-    { iSplit.
-      iPureIntro ; clear -Hflp' Hwa; destruct p0,p'; cbn in *; try done.
-      iFrame "#".
-      destruct (writeAllowed p') eqn:Hwa'; cycle 1.
-      { destruct p0, p'; cbn in *; try congruence;  inv Hflp'. }
-      by iDestruct ("Hwcond'" with "HVstorev1") as "HP'storev".
-    }
-    iDestruct (region_open_prepare with "Hr") as "$".
+      iDestruct (region_close_next with "[$Hr $Ha1 $Hrel' $Hstate' Hmono HmonoV]") as "Hr"; eauto.
+      { intros [g Hcontr]. specialize (H2 g). done. }
+      { apply not_elem_of_cons; split; [auto|apply not_elem_of_nil]. }
+      { iSplit.
+        iPureIntro ; clear -Hflp' Hwa; destruct p0,p'; cbn in *; try done.
+        destruct (writeAllowed p') eqn:Hwa'; cycle 1.
+        { destruct p0, p'; cbn in *; try congruence;  inv Hflp'. }
+        iDestruct ("Hwcond'" with "HVstorev1") as "HP'storev".
+        iFrame "#".
+        iApply monotonicity_guarantees_region_canStore ; auto.
+        destruct p0,p',storev; cbn in *; inv Hflp' ; try congruence.
+        all: destruct (isGlobalSealable sb); done.
+      }
+      iDestruct (region_open_prepare with "Hr") as "$".
     + subst a0. iDestruct "HStoreRes" as "[-> [HStoreRes %]]".
       rewrite insert_insert -memMap_resource_1.
       rewrite lookup_insert in Ha0; inversion Ha0; simplify_eq.
@@ -575,12 +386,6 @@ Qed.
       }
    Qed.
 
-   Lemma if_later {C} {eqdec: Decision C} (Q Q' : iProp Σ) : (if (decide C) then ▷ Q else Q') -∗ ▷ (if (decide C) then Q else Q').
-   Proof. iIntros "H". destruct (decide C);auto. Qed.
-
-   Lemma if_later_bool (b : bool) (Q Q' : iProp Σ) : (if b then ▷ Q else Q') -∗ ▷ (if b then Q else Q').
-   Proof. iIntros "H". destruct b;auto. Qed.
-
   Lemma allow_store_mem_later:
     ∀ (W : WORLD) (regs : leibnizO Reg)
       (a : Addr) (w : Word) r1 r2 (p' : Perm) (mem0 : Mem),
@@ -597,8 +402,8 @@ Qed.
     iDestruct "HStoreRes" as (p0 P w0 Hp'O Hpers) "(#Hzcond & #Hwcond & #Hrcond & -> & HStoreMem)".
     repeat (iApply later_exist_2; iExists _).
     repeat (iApply later_sep_2; iSplitR; auto).
-    iDestruct (if_later_bool with "Hwcond") as "Hwcond'"; eauto.
-    iDestruct (if_later_bool with "Hrcond") as "Hrcond'"; eauto.
+    iDestruct (if_later with "Hwcond") as "Hwcond'"; eauto.
+    iDestruct (if_later with "Hrcond") as "Hrcond'"; eauto.
   Qed.
 
    Lemma store_case (W : WORLD) (regs : leibnizO Reg)
@@ -607,7 +412,7 @@ Qed.
      ftlr_instr W regs p p' g b e a w (Store dst src) ρ P.
    Proof.
     intros Hp Hsome i Hbae Hfp HO Hpers Hpwl Hregion Hnotrevoked Hnotfrozen Hi.
-    iIntros "#IH #Hinv_interp #Hreg #Hinva #Hrcond #Hwcond Hmono Hw Hsts Hown".
+    iIntros "#IH #Hinv_interp #Hreg #Hinva #Hrcond #Hwcond HmonoV Hmono Hw Hsts Hown".
     iIntros "Hr Hstate Ha HPC Hmap".
     (* iDestruct (execCond_implies_region_conditions with "Hinv_interp") as "#Hinv"; eauto. *)
     iInsert "Hmap" PC.
@@ -658,8 +463,7 @@ Qed.
     { rewrite /subseteq /map_subseteq. intros rr _.
       apply elem_of_dom. rewrite lookup_insert_is_Some'; eauto. }
     { iSplitR "Hmap"; auto. }
-    rewrite /wcond.
-    iDestruct (if_later with "Hwcond") as "Hwcond'";auto.
+    iDestruct (if_dec_later with "Hwcond") as "Hwcond'";auto.
     iDestruct (allow_store_mem_later with "HStoreMem") as "HStoreMem".
 
     iNext. iIntros (regs' mem' retv). iDestruct 1 as (HSpec) "[Hmem Hmap]".
@@ -672,19 +476,21 @@ Qed.
       (* From this, derive value relation for the current PC*)
       (* iDestruct (execcPC_implies_interp _ _ _ _ _ a  with "Hinv") as "HVPC"; eauto. *)
 
-      iDestruct (switch_monotonicity_formulation with "Hmono") as "Hmono"; [eauto..|].
+      iDestruct (switch_monotonicity_formulation with "HmonoV") as "HmonoV"; [eauto..|].
+      iDestruct (switch_monotonicityFull_formulation with "Hmono") as "Hmono"; [eauto..|].
 
       (* assert that the PC *)
 
       (* Step 4: return all the resources we had in order to close the second location
          in the region, in the cases where we need to *)
       iDestruct (mem_map_recover_res
-                  with "HStoreMem Hreg Hinv_interp Hw Hrcond [Hwcond] Hmono Hmem")
-        as (w') "(Hr & Ha & HSVInterp & Hmono)"; eauto.
+                  with "HStoreMem Hreg Hinv_interp Hw Hrcond [Hwcond] HmonoV Hmono Hmem")
+        as (w') "(Hr & Ha & HSVInterp & HmonoV & Hmono)"; eauto.
 
-      iDestruct (switch_monotonicity_formulation with "Hmono") as "Hmono"; auto.
+      iDestruct (switch_monotonicity_formulation with "HmonoV") as "HmonoV"; auto.
+      iDestruct (switch_monotonicityFull_formulation with "Hmono") as "Hmono"; auto.
 
-      iDestruct (region_close with "[$Hstate $Hr $Ha $Hmono $HSVInterp]") as "Hr"; eauto.
+      iDestruct (region_close with "[$Hstate $Hr $Ha $HmonoV $Hmono $HSVInterp]") as "Hr"; eauto.
       { destruct ρ;auto;[|ospecialize (Hnotfrozen _)];contradiction. }
       simplify_map_eq. rewrite insert_insert.
 
